test/omega/test.lean
@@ -49,8 +49,7 @@ example {x y : Nat} (_ : 6 * x + 7 * y = 5) : False := by omega
 example {x y : Nat} (_ : x * 6 + y * 7 = 5) : False := by omega
 example {x y : Nat} (_ : 2 * (3 * x) + y * 7 = 5) : False := by omega
 example {x y : Nat} (_ : 2 * x * 3 + y * 7 = 5) : False := by omega
--- Currently fails:
--- example {x y : Nat} (_ : 2 * 3 * x + y * 7 = 5) : False := by omega
+example {x y : Nat} (_ : 2 * 3 * x + y * 7 = 5) : False := by omega
 
 example {x : Nat} (_ : x < 0) : False := by omega
 
